---
title: "Assignment #1"
author: "Boyu, Chen R11323006"
date: "2023-03-16"
output: html_document
---

```{r setup, include=FALSE}
knitr::opts_chunk$set(echo = TRUE)
```

# Q1
The square of Euclidean norm represented by matrix form is 
```{=tex}
\begin{align*}
&\| \beta \|^2_2 = \sum_j |\beta_j|^2\\
&\lambda \| \beta \|^2_2 = \lambda \sum_i |\beta_j|^2 = \lambda \sum_i \beta_j^2 = \beta^T \lambda I \beta
\end{align*}
```
Let $Q$ denote the objective function, $Q = (Y-X\beta)^T(Y-X\beta) + \lambda\| \beta \|^2_2$
```{=tex}
\begin{align*}

\hat\beta &= \mathop{\arg\min}_{\beta}Q \\
&= \mathop{\arg\min}_{\beta} (Y-X\beta)^T(Y-X\beta) + \beta^T \lambda  I\beta\\ 
&= \mathop{\arg\min}_{\beta} Y^TY - 2Y^TX\beta+\beta^TX^TX\beta+ \beta^T \lambda I \beta

\end{align*}
```
By the First-order condition w.r.t.$\beta$, we have
```{=tex}
\begin{align*}
F.O.C. \\
\\
&\frac{\partial Q}{\partial \beta} = -2X^TY+2X^TX\hat\beta+2\lambda I \hat\beta =0\\
& \Rightarrow -X^TY + (X^TX+I)\hat\beta = 0 \\
& \Rightarrow \hat\beta_{Ridge} = (X^TX + \lambda I)^{-1}X^TY
\end{align*}
```


